GeneralReflection.v
@@ -1,0 +1,473 @@
+Require Import MetaCoq.Checker.Checker.
+From MetaCoq.Template Require Import utils All Pretty.
+Require Import List String.
+Import MonadNotation.
+Require Import FOL.
+Require Import Deduction.
+Require Import Tarski.
+Require Import VectorTech.
+Require Import Lia.
+
+Section FailureMonad.
+  (* Our monad for creating proper error messages *)
+  Inductive FailureMonad (A:Type) : Type := ret : A -> FailureMonad A | fail : string -> FailureMonad A.
+  Arguments ret {_} _.
+  Arguments fail {_} _.
+  Definition bind {A B : Type} (k:FailureMonad A) (f:A -> FailureMonad B) := match k return FailureMonad B with fail x => fail x | ret k => f k end.
+  Notation "x <- c1 ;; c2" := (bind c1 (fun x => c2)).
+  Definition f2t {T:Type} (a:FailureMonad T) : TemplateMonad T := match a with ret k => monad_utils.ret k | fail s => tmFail s end.
+  Fixpoint flatten_monad {A:Type} (l:list (FailureMonad A)) : FailureMonad (list A) := match l with nil => ret nil | x::xr => xm <- x;; xrm <- flatten_monad xr;; ret (xm::xrm) end.
+  Definition map_monad {A B:Type} (f:A -> FailureMonad B) (l:list A) : FailureMonad (list B) := flatten_monad (map f l).
+End FailureMonad.
+
+Arguments ret {_} _.
+Arguments fail {_} _.
+Notation "x <- c1 ;; c2" := (bind c1 (fun x => c2)).
+Arguments Vector.cons {_} _ {_} _, _ _ _ _.
+
+Section MetaCoqUtils.
+  (* Working with quoted vectors *)
+  Notation vectorCons x T n xr := 
+  (tApp
+   (tConstruct
+      {|
+      inductive_mind := (MPfile (["VectorDef"; "Vectors"; "Coq"]), "t");
+      inductive_ind := 0 |} 1 nil)
+   ([T; x; n; xr])).
+  Notation vectorNil T :=
+  (tApp
+   (tConstruct
+      {|
+      inductive_mind := (MPfile (["VectorDef"; "Vectors"; "Coq"]), "t");
+      inductive_ind := 0 |} 0 nil) ([T])).
+  Fixpoint recoverVector (f : Ast.term) {struct f}: FailureMonad (list Ast.term) := let ffail := fail "not a vector application" in match f with
+    vectorNil _ => ret nil
+  | vectorCons x _ _ xr => xrl <- recoverVector xr;;ret (x::xrl)
+  | _ => ffail
+  end.
+
+  (* General utils for quoted terms *)
+  Existing Instance config.default_checker_flags.
+  Fixpoint popNElements (l : list Ast.term) (n:nat) : option (list Ast.term) := match (l,n) with
+    (a,0) => Some a
+  | (x::xr, S n) => popNElements xr n
+  | _ => None end.
+  Fixpoint popListStart (l : list Ast.term) (ls : list Ast.term) : option (list Ast.term) := match (l,ls) with
+    (a,nil)=> Some a
+  | (lx::lxr, lsx::lsxr) => if Checker.eq_term init_graph lx lsx then popListStart lxr lsxr else None
+  | _ => None end.
+  MetaCoq Quote Definition qNatZero := 0.
+  MetaCoq Quote Definition qNatSucc := S.
+  MetaCoq Quote Definition qeq_refl := (@eq_refl).
+  Fixpoint quoteNumber (n:nat) : Ast.term:= match n with 0 => qNatZero | S n => tApp qNatSucc ([quoteNumber n]) end.
+
+  Fixpoint addRelIndex (minn:nat) (amnt:nat) (t:Ast.term) : Ast.term := match t with
+    tRel n => if Compare_dec.le_gt_dec minn n then tRel (amnt+n) else tRel n
+  | tVar k => tVar k
+  | tEvar n ls => tEvar n (map (addRelIndex minn amnt) ls)
+  | tSort u => tSort u
+  | tCast t ck t2 => tCast (addRelIndex minn amnt t) ck (addRelIndex minn amnt t2)
+  | tProd n t v => tProd n (addRelIndex minn amnt t) (addRelIndex (S minn) amnt v)
+  | tLambda n t v => tLambda n (addRelIndex minn amnt t) (addRelIndex (S minn) amnt v)
+  | tLetIn n t v e => tLetIn n (addRelIndex minn amnt t) (addRelIndex minn amnt v) (addRelIndex (S minn) amnt e)
+  | tApp f al => tApp (addRelIndex minn amnt f) (map (addRelIndex minn amnt) al)
+  | tConst a b => tConst a b
+  | tInd i t => tInd i t
+  | tConstruct a b c => tConstruct a b c
+  | tCase k i r m => tCase k (addRelIndex minn amnt i) (addRelIndex minn amnt r) (map (fun '(a,b) => (a,addRelIndex minn amnt b)) m)
+  | tProj p t => tProj p (addRelIndex minn amnt t)
+  | tFix mft n => tFix (map (map_def (addRelIndex minn amnt) (addRelIndex (S minn) amnt)) mft) n
+  | tCoFix mft n => tCoFix (map (map_def (addRelIndex minn amnt) (addRelIndex (S minn) amnt)) mft) n
+  end.
+  Definition map_def_monad {A B : Type} (tyf bodyf : A -> FailureMonad B) (d:def A) : FailureMonad (def B) := dtr <- tyf (dbody d);;dbr <- bodyf (dbody d);; 
+                                                                                                            ret {| dname := dname d; dtype := dtr; dbody := dbr; rarg := rarg d |}.
+  Fixpoint lowerRelIndex (minn:nat) (tv:FailureMonad Ast.term) (t:Ast.term) {struct t}: FailureMonad Ast.term := match t with
+    tRel n => if Compare_dec.le_gt_dec minn n then if Compare_dec.le_gt_dec minn (S n) then ret (tRel (match n with 0 => 0 | S n => n end)) else tv else ret (tRel n)
+  | tVar k => ret (tVar k)
+  | tEvar n ls => m <- map_monad (lowerRelIndex minn tv) ls;;ret (tEvar n m)
+  | tSort u => ret (tSort u)
+  | tCast t ck t2 => mt <- (lowerRelIndex minn tv t);;mt2<-(lowerRelIndex minn tv t2);;ret (tCast mt ck mt2)
+  | tProd n t v => mt<-(lowerRelIndex minn tv t);;mv<-(lowerRelIndex (S minn) tv v);;ret (tProd n mt mv)
+  | tLambda n t v => mt<-(lowerRelIndex minn tv t);;mv<-(lowerRelIndex (S minn) tv v);;ret (tLambda n mt mv)
+  | tLetIn n t v e => mt<-(lowerRelIndex minn tv t);;mv<-(lowerRelIndex minn tv v);;me<-(lowerRelIndex (S minn) tv e);;ret (tLetIn n mt mv me)
+  | tApp f al => mal<-(map_monad (lowerRelIndex minn tv) al);;ff <- lowerRelIndex minn tv f;;ret (tApp ff mal)
+  | tConst a b => ret (tConst a b)
+  | tInd i t => ret (tInd i t)
+  | tConstruct a b c => ret (tConstruct a b c)
+  | tCase k i r m => mi<-(lowerRelIndex minn tv i);;mr<-(lowerRelIndex minn tv r);;mm<-(map_monad (fun '(a,b) => mb <- lowerRelIndex minn tv b;; ret (a,mb)) m);;ret (tCase k mi mr mm)
+  | tProj p t => mt<-(lowerRelIndex minn tv t);;ret (tProj p mt)
+  | tFix mft n => mmft<-(map_monad (map_def_monad (lowerRelIndex minn tv) (lowerRelIndex (S minn) tv)) mft);;ret (tFix mmft n)
+  | tCoFix mft n => mmft<-(map_monad (map_def_monad (lowerRelIndex minn tv) (lowerRelIndex (S minn) tv)) mft);;ret (tCoFix mmft n)
+  end.
+End MetaCoqUtils.
+
+Section AbstractReflectionDefinitions.
+  Class tarski_reflector := {
+  fs : funcs_signature;
+  ps : preds_signature;
+  D  : Type;
+  I  : @interp fs ps D;
+  emptyEnv : nat -> D;
+  isD : Ast.term -> bool
+  }. 
+
+  Context {tr : tarski_reflector}.
+  Fixpoint naryProp (n:nat) : Type := match n with 0 => Prop | S nn => D -> naryProp nn end.
+  Fixpoint representsP {n:nat} phi rho : (forall (P:naryProp n), Prop) := match n return (forall (P:naryProp n), Prop) with
+       0  => (fun (P:Prop) => P <-> @sat fs ps D I rho phi)
+    | S n => (fun (P:D -> naryProp n) => forall d, @representsP n phi (d.:rho) (P d)) end.
+  Definition representableP (n:nat) (P : naryProp n) := exists phi rho, representsP phi rho P.
+  Definition representsF (d:D) trm rho := @eval fs ps D I rho trm = d.
+  Definition representableF (d:D) := exists trm rho, representsF d trm rho.
+
+  Fixpoint naryGFunc (n:nat) (A R : Type) := match n with 0 => R | S n => A -> @naryGFunc n A R end.
+  Fixpoint takeMultiple {n : nat} (X Y:Type)  : (Vector.t X n -> Y) -> @naryGFunc n X Y := 
+     match n as nn return (Vector.t X nn -> Y) -> @naryGFunc nn X Y
+             with 0 => fun R => R (Vector.nil X) 
+              | S n => fun R v => @takeMultiple n X Y (fun vr => R (Vector.cons X v n vr)) end.
+  Definition constructTerm (k:@syms (@fs tr)) := @takeMultiple (ar_syms k) term term (func k).
+  Definition constructForm (k:(@preds (@ps tr))) := @takeMultiple (@ar_preds (@ps tr) k) (@term (@fs tr)) form (atom k).
+
+  Fixpoint nary3GFunc (n:nat) (A B A' B':Type) (C:A -> B -> Type) (C':A'->B'->Type) : (Vector.t A n -> A') -> (Vector.t B n -> B') -> Type
+                      := match n with 0 => fun mA mB => C' (mA (Vector.nil A)) (mB (Vector.nil B))
+                                  | S n => fun mA mB => forall (a:A) (b:B), C a b -> @nary3GFunc n A B A' B' C C' (fun v => mA (Vector.cons A a n v)) (fun v => mB (Vector.cons B b n v)) end.
+
+  Definition mergeTermBase (c:@syms (@fs tr)) : Type := 
+  forall (rho:nat -> D), @nary3GFunc (ar_syms c) term D term D 
+                                     (fun t d => representsF d t rho) (fun t d => representsF d t rho) 
+                                     (func c) (@i_f fs ps D I c).
+  Definition mergeTermProtoType (rho:nat -> D) (n:nat) (fZ:vec term n -> term) (ifZ : vec D n -> D) := 
+         (forall v : vec term n, @eval fs ps D I rho (fZ v) = ifZ (Vector.map (@eval fs ps D I rho) v))  
+         -> @nary3GFunc n term D term D (fun t d => representsF d t rho) (fun t d => representsF d t rho) fZ ifZ.
+  Definition mergeTermProto (rho:nat -> D) (n:nat) (fZ:vec term n -> term) (ifZ : vec D n -> D) : mergeTermProtoType rho n fZ ifZ.
+  Proof.
+  intros H. induction n as [|n IH].
+  * cbn. unfold representsF. rewrite H. cbn. easy.
+  * cbn. intros t d r. apply IH. cbn. intros v. specialize (H (Vector.cons t v)). unfold representsF in r. rewrite H. cbn. now rewrite r.
+  Defined.
+  Definition mergeTerm (c:syms) : mergeTermBase c.
+  Proof. intros rho. eapply mergeTermProto. now intros v. Defined.
+
+  Definition mergeFormBase (c:@preds (@ps tr)) : Type := 
+  forall (rho:nat -> D), @nary3GFunc (ar_preds c) term D form (naryProp 0) 
+                                     (fun t d => representsF d t rho) (fun t P => representsP t rho P) 
+                                     (atom c) (@i_P fs ps D I c).
+  Definition mergeFormProtoType (rho:nat -> D) (n:nat) (fZ:vec term n -> form) (ifZ : vec D n -> naryProp 0) := 
+         (forall v : vec term n, @sat fs ps D I rho (fZ v) = ifZ (Vector.map (@eval fs ps D I rho) v))  
+         -> @nary3GFunc n term D form (naryProp 0) (fun t d => representsF d t rho) (fun t P => representsP t rho P) fZ ifZ.
+  Definition mergeFormProto (rho:nat -> D) (n:nat) (fZ:vec term n -> form) (ifZ : vec D n -> naryProp 0) : mergeFormProtoType rho n fZ ifZ.
+  Proof.
+  intros H. induction n as [|n IH].
+  * cbn. unfold representsP. rewrite H. cbn. easy.
+  * cbn. intros t d r. apply IH. cbn. intros v. specialize (H (Vector.cons t v)). unfold representsF in r. rewrite H. cbn. now rewrite r.
+  Defined.
+  Definition mergeForm (c:preds) : mergeFormBase c.
+  Proof. intros rho. eapply mergeFormProto. now intros v. Defined.
+  MetaCoq Quote Definition qConstructTerm := constructTerm.
+  MetaCoq Quote Definition qMergeTerm := mergeTerm.
+  MetaCoq Quote Definition qConstructForm := constructForm.
+  MetaCoq Quote Definition qMergeForm := mergeForm.
+
+End AbstractReflectionDefinitions.
+
+Section TarskiMerging.
+  Context {tr : tarski_reflector}.
+  Definition mergeFalse (rho:nat -> D) : @representsP tr 0 fal rho False.
+  Proof. easy. Defined.
+  MetaCoq Quote Definition qMergeFalse := @mergeFalse.
+  Definition mFalse := (@fal fs ps full_operators).
+  MetaCoq Quote Definition qMergeFormFalse := @mFalse.
+
+  Definition mergeAnd (rho:nat -> D) (P Q : naryProp 0) (fP fQ : form) : representsP fP rho P -> representsP fQ rho Q -> @representsP tr 0 (fP∧fQ) rho (P /\ Q).
+  Proof.
+  intros [pPl pPr] [pQl pQr]. split.
+  * intros [pP pQ]. split. now apply pPl. now apply pQl.
+  * intros [pP pQ]. split. now apply pPr. now apply pQr.
+  Defined.
+  MetaCoq Quote Definition qMergeAnd := @mergeAnd.
+  Definition mAnd := (@bin fs ps full_operators Conj).
+  MetaCoq Quote Definition qMergeFormAnd := @mAnd.
+
+  Definition mergeOr (rho:nat -> D) (P Q : naryProp 0) (fP fQ : form) : representsP fP rho P -> representsP fQ rho Q -> @representsP tr 0 (fP∨fQ) rho (P \/ Q).
+  Proof.
+  intros [pPl pPr] [pQl pQr]. split.
+  * intros [pP|pQ]. left; now apply pPl. right; now apply pQl.
+  * intros [pP|pQ]. left; now apply pPr. right; now apply pQr.
+  Defined.
+  MetaCoq Quote Definition qMergeOr := @mergeOr.
+  Definition mOr := (@bin fs ps full_operators Disj).
+  MetaCoq Quote Definition qMergeFormOr := @mOr.
+
+  Definition mergeExists (rho:nat -> D) (P:naryProp 1) (fP:form) : representsP fP rho P -> @representsP tr 0 (∃ fP) rho (exists q:D, P q).
+  Proof.
+  intros pR. split.
+  * intros [q Pq]. exists q. destruct (pR q) as [pRl pRr]. now apply pRl.
+  * intros [q Pq]. exists q. destruct (pR q) as [pRl pRr]. now apply pRr.
+  Defined.
+  MetaCoq Quote Definition qMergeExists := @mergeExists.
+  Definition mExists := (@quant fs ps full_operators Ex).
+  MetaCoq Quote Definition qMergeFormExists := @mExists.
+
+  Definition mergeImpl (rho:nat -> D) (P Q : naryProp 0) (fP fQ : form) : representsP fP rho P -> representsP fQ rho Q -> @representsP tr 0 (fP --> fQ) rho (P -> Q).
+  Proof.
+  intros HP HQ.
+  destruct HP as [pPl pPr]. destruct HQ as [pQl pQr]. split.
+  * intros PQ pP. apply pQl, PQ, pPr, pP.
+  * cbn. intros pPQ pP. apply pQr, pPQ, pPl, pP.
+  Defined.
+  MetaCoq Quote Definition qMergeImpl := @mergeImpl.
+  Definition mImpl := (@bin fs ps full_operators Impl).
+  MetaCoq Quote Definition qMergeFormImpl := @mImpl.
+
+  Definition mergeForall (rho:nat -> D) (Q:naryProp 1) (phi:form) : representsP phi rho Q -> @representsP tr 0 (∀ phi) rho (forall x:D, Q x).
+  Proof. intros H. cbn. split;
+   intros HH d; specialize (HH d); specialize (H d); cbn in H; apply H, HH.
+  Defined.
+  MetaCoq Quote Definition qMergeForall := @mergeForall.
+  Definition mForall := (@quant fs ps full_operators All).
+  MetaCoq Quote Definition qMergeFormForall := @mForall.
+
+  Notation baseLogicConn x l:= (tInd {| inductive_mind := (MPfile (["Logic"; "Init"; "Coq"]), x); inductive_ind := 0 |} l).
+  Definition baseConnectiveReifier := Ast.term -> list Ast.term -> nat -> Ast.term -> (Ast.term -> FailureMonad nat) -> (Ast.term -> nat -> Ast.term -> (Ast.term -> FailureMonad nat) -> FailureMonad (prod Ast.term Ast.term))-> FailureMonad (prod Ast.term Ast.term).
+  Definition reifyAnd : baseConnectiveReifier := fun tct lst _ envTerm env fPR => match lst with [x; y] => 
+                                             xr <- fPR x 0 envTerm env;;yr <- fPR y 0 envTerm env;; let '((xt,xp),(yt,yp)) := (xr,yr) in
+                                             ret (tApp qMergeFormAnd ([tct;xt;yt]), tApp qMergeAnd ([tct;envTerm;x;y;xt;yt;xp;yp])) | _ => fail "And applied to != 2 terms" end.
+  Definition reifyOr  : baseConnectiveReifier := fun tct lst _ envTerm env fPR => match lst with [x; y] => 
+                                             xr <- fPR x 0 envTerm env;;yr <- fPR y 0 envTerm env;; let '((xt,xp),(yt,yp)) := (xr,yr) in
+                                             ret (tApp qMergeFormOr ([tct;xt;yt]),tApp qMergeOr ([tct;envTerm;x;y;xt;yt;xp;yp])) | _ => fail "Or applied to != 2 terms" end.
+  Definition reifyExist:baseConnectiveReifier := fun tct lst _ envTerm env fPR => match lst with [_; P] => 
+                                             rr <- fPR P 1 envTerm env;; let '(rt,rp) := rr in 
+                                             ret (tApp qMergeFormExists ([tct;rt]), tApp qMergeExists ([tct;envTerm;P;rt;rp])) | _ => fail "Exist applied to wrong terms" end.
+  Definition reifyBase (s:string) : baseConnectiveReifier := match s with "and" => reifyAnd | "or" => reifyOr | "ex" => reifyExist | _ => fun _ _ _ _ _ _ => fail ("Unknown connective "++s) end.
+
+  Definition baseConnectiveReifierNP := Ast.term -> list Ast.term -> nat -> Ast.term -> (Ast.term -> FailureMonad nat) -> (Ast.term -> nat -> Ast.term -> (Ast.term -> FailureMonad nat) -> FailureMonad ( Ast.term))-> FailureMonad (Ast.term).
+  Definition reifyAndNP : baseConnectiveReifierNP := fun tct lst _ envTerm env fPR => match lst with [x; y] => 
+                                             xt <- fPR x 0 envTerm env;;yt <- fPR y 0 envTerm env;; 
+                                             ret (tApp qMergeFormAnd ([tct;xt;yt])) | _ => fail "And applied to != 2 terms" end.
+  Definition reifyOrNP  : baseConnectiveReifierNP := fun tct lst _ envTerm env fPR => match lst with [x; y] => 
+                                             xt <- fPR x 0 envTerm env;;yt <- fPR y 0 envTerm env;; 
+                                             ret (tApp qMergeFormOr ([tct;xt;yt])) | _ => fail "Or applied to != 2 terms" end.
+  Definition reifyExistNP:baseConnectiveReifierNP := fun tct lst _ envTerm env fPR => match lst with [_; P] => 
+                                             rt <- fPR P 1 envTerm env;;
+                                             ret (tApp qMergeFormExists ([tct;rt])) | _ => fail "Exist applied to wrong terms" end.
+  Definition reifyBaseNP (s:string) : baseConnectiveReifierNP := match s with "and" => reifyAndNP | "or" => reifyOrNP | "ex" => reifyExistNP | _ => fun _ _ _ _ _ _ => fail ("Unknown connective "++s) end.
+
+End TarskiMerging.
+
+Section ReificationHelpers.
+  Definition termReifier := Ast.term -> list Ast.term -> Ast.term -> (Ast.term -> FailureMonad (prod Ast.term Ast.term)) -> FailureMonad (prod Ast.term Ast.term).
+  Definition termReifierNP := Ast.term -> list Ast.term -> Ast.term -> (Ast.term -> FailureMonad (Ast.term)) -> FailureMonad (Ast.term).
+  (* typeClassTerm -> vector of args -> env term -> recursion for arg vector -> prod (term, proof that term represents input *)
+  Fixpoint applyRecursively (lt : list Ast.term) (IH : Ast.term -> FailureMonad (prod Ast.term Ast.term)) : FailureMonad (prod (list Ast.term) (list Ast.term)) :=
+     match lt with nil => ret (nil,nil)
+               | t::tr => IHt <- IH t;; atrIH <- applyRecursively tr IH;;let '(rep,prf) := IHt in let '(replist,fulllist) := atrIH in ret (rep::replist, rep::t::prf::fulllist) end.
+  Fixpoint applyRecursivelyNP (lt : list Ast.term) (IH : Ast.term -> FailureMonad (Ast.term)) : FailureMonad ((list Ast.term) ) :=
+     match lt with nil => ret (nil)
+               | t::tr => rep <- IH t;; replist <- applyRecursivelyNP tr IH;;ret (rep::replist) end.
+  Definition reifyTerm (c:Ast.term) : termReifier := fun tct av env IH => pr <- applyRecursively av IH;; let '(trm,fullarg) := pr in
+                                                     ret (tApp qConstructTerm (tct::c::trm), tApp qMergeTerm (tct::c::env::fullarg)).
+  Definition reifyForm (c:Ast.term) : termReifier := fun tct av env IH => pr <- applyRecursively av IH;; let '(trm,fullarg) := pr in
+                                                     ret (tApp qConstructForm (tct::c::trm), tApp qMergeForm (tct::c::env::fullarg)).
+  Definition reifyTermNP (c:Ast.term) : termReifierNP := fun tct av env IH => trm <- applyRecursivelyNP av IH;; 
+                                                     ret (tApp qConstructTerm (tct::c::trm)).
+  Definition reifyFormNP (c:Ast.term) : termReifierNP := fun tct av env IH => trm <- applyRecursivelyNP av IH;; 
+                                                     ret (tApp qConstructForm (tct::c::trm)).
+    
+End ReificationHelpers.
+
+Section EnvHelpers.
+  Definition appendZero (env:Ast.term -> FailureMonad nat) (zv:FailureMonad nat) : (Ast.term -> FailureMonad nat) := 
+        fun (t:Ast.term) => match t with tRel n => (match n with 0 => zv | S n => env (tRel n) end) | _ => k <- lowerRelIndex 0 (fail "tRel 0 used when lowering") t;; (env k) end.
+  Definition appendAndLift (env:Ast.term -> FailureMonad nat) (zv:FailureMonad nat) : (Ast.term -> FailureMonad nat) := 
+        fun t => match t with tRel n => (match n with 0 => zv | S n => k <- env (tRel n);;ret (S k) end) | _ => k <- lowerRelIndex 0 (fail "tRel 0 used when lowering") t;; v <- env k;;ret (S v) end.
+  MetaCoq Quote Definition qD := @D.
+  MetaCoq Quote Definition qScons := @scons.
+  Definition raiseEnvTerm (tct:Ast.term) (d:Ast.term) (env:Ast.term) : Ast.term := tApp (qScons) ([tApp qD ([tct]);d;env]).
+  Definition unboundEnv := (fun a:Ast.term => @fail nat ("unbound " ++ string_of_term a)).
+End EnvHelpers.
+
+Section EnvConstructor.
+  Existing Instance config.default_checker_flags.
+  MetaCoq Quote Definition qFs := @fs.
+  MetaCoq Quote Definition qLocalVar := @var.
+  MetaCoq Quote Definition qI_f := @i_f.
+  MetaCoq Quote Definition qI_P := @i_P.
+
+  Fixpoint findUBRecursively (lt : list Ast.term) (IH : Ast.term -> FailureMonad (list Ast.term)) : FailureMonad ((list Ast.term) ) :=
+       match lt with nil => ret (nil)
+                 | t::tr => rep <- IH t;; replist <- findUBRecursively tr IH;;ret (rep++replist) end.
+  
+  Fixpoint findUnboundVariablesTerm (fuel:nat) (t:Ast.term) {struct fuel}: (FailureMonad (list Ast.term)) := 
+    let ffail := ret ([t]) in match fuel with 
+      0 => fail "Out of fuel" 
+      | S fuel => match t with
+          tApp arg l => if Checker.eq_term init_graph arg qI_f then match popNElements l 4 with (*4 for funcs, preds, domain, interp *)
+            Some ([fnc;v]) => vr <- recoverVector v;;findUBRecursively vr (findUnboundVariablesTerm fuel)
+           | _ => ffail end else ffail
+        | _ => ffail
+      end 
+    end.
+
+    Notation baseLogicConn x l:= (tInd {| inductive_mind := (MPfile (["Logic"; "Init"; "Coq"]), x); inductive_ind := 0 |} l).
+    Definition baseUBVarFinder := list Ast.term -> (Ast.term->nat->FailureMonad (list Ast.term)) -> FailureMonad (list Ast.term).
+    Definition findUBAnd  :baseUBVarFinder := fun lst fPR => match lst with [x; y] => 
+                                               xt <- fPR x 0;;yt <- fPR y 0;; 
+                                               ret (xt++yt) | _ => fail "And applied to != 2 terms" end.
+    Definition findUBOr   :baseUBVarFinder := fun lst fPR => match lst with [x; y] => 
+                                               xt <- fPR x 0;;yt <- fPR y 0;; 
+                                               ret (xt++yt) | _ => fail "Or applied to != 2 terms" end.
+    Definition findUBExists:baseUBVarFinder := fun lst fPR => match lst with [_; P] => fPR P 1 | _ => fail "Exist applied to wrong terms" end.
+    Definition findUBBase (s:string) : baseUBVarFinder := match s with "and" => findUBAnd | "or" => findUBOr | "ex" => findUBExists | _ => fun _ _ => fail ("Unknown connective "++s) end.
+
+    Context {tr : tarski_reflector}.
+    Definition maybeD : Ast.term -> Ast.term -> bool := fun tct mD => if @isD tr mD then true else Checker.eq_term init_graph mD (tApp qD ([tct])).
+    Fixpoint findUnboundVariablesForm (tct:Ast.term) (fuel:nat) (t:Ast.term) (frees:nat) {struct fuel}: (FailureMonad (list Ast.term)) := 
+    let ffail := fail ("Cannot introspect form " ++ string_of_term t) in match fuel with 0 => fail "Out of fuel" | S fuel => 
+      match (frees,t) with
+      (0,(baseLogicConn "False" nil)) => ret (nil)
+    | (0,(tApp (baseLogicConn name nil) lst)) => findUBBase name lst (findUnboundVariablesForm tct fuel)
+    | (0,(tApp arg lst)) => if Checker.eq_term init_graph arg qI_P then match popNElements lst 4 with
+            Some ([fnc;v]) => vr <- recoverVector v;;findUBRecursively vr (fun t => findUnboundVariablesTerm fuel t)
+          | _ => ffail end else ffail
+    | (0,tProd x P Q) => if maybeD tct (P) then
+                              findUnboundVariablesForm tct fuel (tLambda x P Q) 1
+                         else
+                              rP <- findUnboundVariablesForm tct fuel P 0;;
+                              Ql <- lowerRelIndex 0 (fail "Used var of implication precondition") Q;;
+                              rQ <- findUnboundVariablesForm tct fuel Ql 0;;
+                              ret (rP++rQ)
+    | (S n,tLambda x T P) => if maybeD tct T then
+          findUnboundVariablesForm tct fuel P n
+         else ffail
+    | _ => ffail end end.
+
+   Fixpoint createEnvTerms (tct:Ast.term) (l:list Ast.term) (base:Ast.term) : prod (Ast.term) (Ast.term -> FailureMonad nat) := match l with 
+         nil => (base,unboundEnv)
+     | x::xr => let '(envTerm,env) := createEnvTerms tct xr base in (raiseEnvTerm tct x envTerm, fun a:Ast.term => if Checker.eq_term init_graph x a then ret 0 else v <- env a;;ret (S v)) end.
+
+
+End EnvConstructor.
+
+Section MainReificationFunctions.
+  Existing Instance config.default_checker_flags.
+  Fixpoint findTermRepresentation (tct:Ast.term) (fuel:nat) (t:Ast.term) (termEnv:Ast.term) (env:Ast.term -> FailureMonad nat) {struct fuel}: (FailureMonad (prod Ast.term Ast.term)) := 
+    let ffail := (envv <- env (t);;let num := quoteNumber (envv) in ret (tApp qLocalVar ([tApp qFs ([tct]);num]),tApp qeq_refl ([tApp qD ([tct]);t]))) in match fuel with 
+      0 => fail "Out of fuel" 
+      | S fuel => match t with
+          tApp arg l => if Checker.eq_term init_graph arg qI_f then match popNElements l 4 with (*4 for funcs, preds, domain, interp *)
+            Some ([fnc;v]) => vr <- recoverVector v;;reifyTerm fnc tct vr termEnv (fun t => findTermRepresentation tct fuel t termEnv env)
+           | _ => ffail end else ffail
+        | _ => ffail
+      end 
+    end.
+
+  Fixpoint findTermRepresentationNP (tct:Ast.term) (fuel:nat) (t:Ast.term) (termEnv:Ast.term) (env:Ast.term -> FailureMonad nat) {struct fuel}: (FailureMonad (Ast.term)) := 
+    let ffail := (envv <- env (t);;let num := quoteNumber (envv) in ret (tApp qLocalVar ([tApp qFs ([tct]);num]))) in match fuel with 
+      0 => fail "Out of fuel" 
+      | S fuel => match t with
+          tApp arg l => if Checker.eq_term init_graph arg qI_f then match popNElements l 4 with (*4 for funcs, preds, domain, interp *)
+            Some ([fnc;v]) => vr <- recoverVector v;;reifyTermNP fnc tct vr termEnv (fun t => findTermRepresentationNP tct fuel t termEnv env)
+           | _ => ffail end else ffail
+        | _ => ffail
+      end 
+    end.
+
+    Notation baseLogicConn x l:= (tInd {| inductive_mind := (MPfile (["Logic"; "Init"; "Coq"]), x); inductive_ind := 0 |} l).
+
+
+    Context {tr : tarski_reflector}.
+    Fixpoint findPropRepresentation (tct:Ast.term) (fuel:nat) (t:Ast.term) (frees:nat) (envTerm:Ast.term) (env:Ast.term -> FailureMonad nat) {struct fuel}: (FailureMonad (prod Ast.term Ast.term)) := 
+    let ffail :=fail ("Cannot represent form " ++ string_of_term t) in match fuel with 0 => fail "Out of fuel" | S fuel => 
+      match (frees,t) with
+      (0,(baseLogicConn "False" nil)) => ret (tApp qMergeFormFalse ([tct]), tApp qMergeFalse ([tct;envTerm]))
+    | (0,(tApp (baseLogicConn name nil) lst)) => reifyBase name tct lst fuel envTerm env (findPropRepresentation tct fuel)
+    | (0,(tApp arg lst)) => if Checker.eq_term init_graph arg qI_P then match popNElements lst 4 with
+            Some ([fnc;v]) => vr <- recoverVector v;;reifyForm fnc tct vr envTerm (fun t => findTermRepresentation tct fuel t envTerm env)
+          | _ => ffail end else ffail
+    | (0,tProd x P Q) => if maybeD tct (P) then
+                              rQ <- findPropRepresentation tct fuel (tLambda x P Q) 1 envTerm env;; let '(tQ,pQ) := rQ in
+                              ret (tApp qMergeFormForall ([tct;tQ]), tApp qMergeForall ([tct;envTerm;tLambda x P Q;tQ;pQ]))
+                         else
+                              rP <- findPropRepresentation tct fuel P 0 envTerm env;;
+                              Ql <- lowerRelIndex 0 (fail "Used var of implication precondition") Q;;
+                              rQ <- findPropRepresentation tct fuel Ql 0 envTerm env;; let '((tP,pP),(tQ,pQ)) := (rP,rQ) in
+                              ret (tApp qMergeFormImpl ([tct;tP;tQ]), tApp qMergeImpl ([tct;envTerm;P;Ql;tP;tQ;pP;pQ]))
+    | (S n,tLambda x T P) => if maybeD tct T then
+          let envTermSub := raiseEnvTerm tct (tRel 0) (addRelIndex 0 1 envTerm) in
+          let envSub := appendAndLift env (ret 0) in
+          k <- findPropRepresentation tct fuel P n envTermSub envSub;; let '(tk,pk) := k in
+          ret (tk,(tLambda x (tApp qD ([tct])) pk))
+         else ffail
+    | _ => ffail end end.
+
+    Fixpoint findPropRepresentationNP (tct:Ast.term) (fuel:nat) (t:Ast.term) (frees:nat) (envTerm:Ast.term) (env:Ast.term -> FailureMonad nat) {struct fuel}: (FailureMonad (Ast.term)) := 
+    let ffail :=fail ("Cannot represent form " ++ string_of_term t) in match fuel with 0 => fail "Out of fuel" | S fuel => 
+      match (frees,t) with
+      (0,(baseLogicConn "False" nil)) => ret (tApp qMergeFormFalse ([tct]))
+    | (0,(tApp (baseLogicConn name nil) lst)) => reifyBaseNP name tct lst fuel envTerm env (findPropRepresentationNP tct fuel)
+    | (0,(tApp arg lst)) => if Checker.eq_term init_graph arg qI_P then match popNElements lst 4 with
+            Some ([fnc;v]) => vr <- recoverVector v;;reifyFormNP fnc tct vr envTerm (fun t => findTermRepresentationNP tct fuel t envTerm env)
+          | _ => ffail end else ffail
+    | (0,tProd x P Q) => if maybeD tct (P) then
+                              tQ <- findPropRepresentationNP tct fuel (tLambda x P Q) 1 envTerm env;; 
+                              ret (tApp qMergeFormForall ([tct;tQ]))
+                         else
+                              tP <- findPropRepresentationNP tct fuel P 0 envTerm env;;
+                              Ql <- lowerRelIndex 0 (fail "Used var of implication precondition") Q;;
+                              tQ <- findPropRepresentationNP tct fuel Ql 0 envTerm env;; 
+                              ret (tApp qMergeFormImpl ([tct;tP;tQ]))
+    | (S n,tLambda x T P) => if maybeD tct T then
+          let envTermSub := raiseEnvTerm tct (tRel 0) (addRelIndex 0 1 envTerm) in
+          let envSub := appendAndLift env (ret 0) in
+          tk <- findPropRepresentationNP tct fuel P n envTermSub envSub;;
+          ret (tk)
+         else ffail
+    | _ => ffail end end.
+
+  
+End MainReificationFunctions.
+
+
+Definition FUEL := 100. 
+Ltac representEnvP env1 env2:= 
+match goal with [ |- @representableP ?i ?n ?G ] =>
+  let rep := fresh "rep" in let prf := fresh "prf" in let env := fresh "env" in let k y := (destruct y as [rep prf]) in
+  pose ((match env1 with None => @emptyEnv i | Some kk => kk end)) as env;
+  (run_template_program (monad_utils.bind (tmQuote i) (fun tct =>
+                         monad_utils.bind (tmQuote G) (fun g => 
+                         monad_utils.bind (tmQuote env) (fun qe => 
+                         monad_utils.bind (f2t (@findPropRepresentation i tct FUEL g n qe env2)) (fun '(tPq,pPq) => 
+                         monad_utils.bind (tmUnquoteTyped (form) tPq) (fun tP:form => 
+                         monad_utils.bind (tmUnquoteTyped (@representsP i n tP env G) pPq) (fun tQ : @representsP i n tP env G =>
+                         monad_utils.ret (@existT form (fun mm => @representsP i n mm env G) tP tQ)))))))) k)
+  ;exists rep;exists env;exact prf 
+end.
+
+
+Ltac representEnvPNP env1 env2:= 
+match goal with [ |- @representableP ?i ?n ?G ] =>
+  let rep := fresh "rep" in let prf := fresh "prf" in let env := fresh "env" in let k y := (pose y as rep) in
+  pose ((match env1 with None => @emptyEnv i | Some kk => kk end)) as env;
+  (run_template_program (monad_utils.bind (tmQuote i) (fun tct =>
+                         monad_utils.bind (tmQuote G) (fun g => 
+                         monad_utils.bind (tmQuote env) (fun qe => 
+                         monad_utils.bind (f2t ((@findPropRepresentationNP i tct FUEL g n qe env2))) (fun tPq => 
+                         monad_utils.bind (tmUnquoteTyped (form) tPq) (fun tP:form => 
+                         monad_utils.ret (tP))))))) k)
+  ;exists rep;exists env;easy 
+end.
+Ltac represent := match goal with [ |- @representableP ?i ?n ?G ] => representEnvP (@None(nat -> @D i)) unboundEnv end.
+Ltac representNP := match goal with [ |- @representableP ?i ?n ?G ] => representEnvPNP (@None(nat -> @D i)) unboundEnv end.
+
+Ltac constructEnv := 
+match goal with [ |- @representableP ?i ?n ?G ] =>
+  let envBase := fresh "envBase" in let envTerm := fresh "envTerm" in let k y := (pose (fst y) as envBase;pose (snd y) as envTerm) in
+  (run_template_program (monad_utils.bind (tmQuote i) (fun tct =>
+                         monad_utils.bind (tmQuote G) (fun g => 
+                         monad_utils.bind (tmQuote (@emptyEnv i)) (fun baseEnv => 
+                         monad_utils.bind (f2t ((@findUnboundVariablesForm i tct FUEL g n))) (fun lst => 
+                         let '(envToDR,envToNat) := (createEnvTerms tct lst baseEnv) in
+                         monad_utils.bind (tmUnquoteTyped (nat -> @D i) envToDR) (fun envToD => 
+                         monad_utils.ret (pair envToD envToNat))))))) k)
+end.
+
